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Chapter 1

Mathematical Introduction

Exercise 1. The null vector is (0, 0, 0). The inverse under addition is (−a,−b,−c). A vector of the form
(a, b, 1) does not form a vector space because it fails to satisfy the closure property under addition and
multiplication:

(a, b, 1) + (d, e, 1) = (a+ d, b+ e, 2) /∈ (a, b, 1)

α(a, b, 1) = (αa, αb, α) /∈ (a, b, 1)

Exercise 2.

Exercise 3. The set of kets is not linearly independent, as |3⟩ = |1⟩ − 2 |2⟩.

Exercise 4. Arrange the row vectors into a matrix and find the determinant:∣∣∣∣∣∣
1 1 0
1 0 1
3 2 1

∣∣∣∣∣∣ = 0

Since the determinant is zero, one of the row vectors is expressible as a linear combination of the others. This
is seen in (3, 2, 1) = 2(1, 1, 0) + (1, 0, 1).

For the second set of vectors, we perform the same procedure:∣∣∣∣∣∣
1 1 0
1 0 1
0 1 1

∣∣∣∣∣∣ = 2

So there is no vector in this set that is expressible as a linear combination of the other vectors.

Exercise 5. Let |I⟩ = A⃗ and |II⟩ = B⃗. Following Gram-Schmidt orthonormalisation:

Â =
3

5
î+

4

5
ĵ = |1⟩

|2′⟩ = |II⟩ − |1⟩ ⟨1|II⟩ = 18

5

1
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Exercise 6.

Exercise 7.



Chapter 2

Review of Classical Mechanics

Exercise 1. The Lagrangian of the system is:

L =
1

2
mẋ2 − 1

2
kx2

Solving the Euler-Lagrange equation gives the equation of motion:

d

dt

∂L
∂ẋ

− ∂L
∂x

= mẍ+ kx = 0

Exercise 2. The Lagrangian of the system is:

L =
1

2
mẋ21 +

1

2
mẋ22 −

1

2
k(x21 + x22)−

1

2
k(x1 − x2)

2

Solving the Euler-Lagrange equations gives the equations of motion:

d

dt

∂L
∂ẋ1

− ∂L
∂x1

= mẍ1 + 2kx1 − kx2 = 0

d

dt

∂L
∂ẋ2

− ∂L
∂x2

= mẍ2 + 2kx2 − kx1 = 0

Rearranging, we get the same equations of motion:

ẍ1 = −2k

m
x1 +

k

m
x2

ẍ2 =
k

m
x1 −

2k

m
x2

Exercise 3. The Lagrangian in polar coordinates is:

L =
1

2
m|ṙ|2 − V (r) =

1

2
m
[
ṙ2 + r2θ̇2 + (r2 sin2 θ)ϕ̇2

]
− V (r)

3
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Solving the Euler-Lagrange equations gives the equations of motion:

d

dt

∂L
∂ṙ

− ∂L
∂r

= mr̈ −mrθ̇2 − (mr sin2 θ)ϕ̇2 +
∂V

∂r
= 0

d

dt

∂L
∂θ̇

− ∂L
∂θ

= mr2θ̈ + 2mrṙθ̇ − 1

2
(mr2 sin 2θ)ϕ̇2 = 0

d

dt

∂L
∂ϕ̇

− ∂L
∂ϕ

= (mr2 sin2 θ)ϕ̈+ 2mϕ̇(rṙ sin2 θ + r2θ̇ sin 2θ) = 0

Exercise 4. Substituting ṙ1 and ṙ2 with ṙCM and ṙ:

L =
1

2
m1

∣∣∣∣ṙCM +
m2ṙ

m1 +m2

∣∣∣∣2 + 1

2
m2

∣∣∣∣ṙCM − m1ṙ

m1 +m2

∣∣∣∣2 − V (r)

Expanding the squares:

L =
1

2
(m1 +m2) |ṙCM|2 + 1

2
m1

∣∣∣∣2m2ṙrCM

m1 +m2

∣∣∣∣+ 1

2
m1

(
m2

m1 +m2

)2

|ṙ|2

−1

2
m2

∣∣∣∣2m1ṙrCM

m1 +m2

∣∣∣∣+ 1

2
m2

(
m1

m1 +m2

)2

|ṙ|2 − V (r) (2.1)

Which gives the final expression:

L =
1

2
(m1 +m2) |ṙCM|2 + 1

2

m1m2

m1 +m2
|ṙ|2 − V (r)

Exercise 5.

Exercise 6. The conservation of energy in the harmonic oscillator states that:

p2

2m
+

1

2
kx2 = E

Dividing both sides by E:

p2

2mE
+
kx2

2E
= 1 −→

(x
a

)2
+
(p
b

)2
= 1, a2 =

2E

k
, b2 = 2mE

Exercise 7. The Lagrangian of the system is:

L =
1

2
mẋ21 +

1

2
mẋ22 −

1

2
k(x21 + x22)−

1

2
k(x1 − x2)

2

Finding the generalised momenta:

pi =
∂L
∂ẋi

= miẋi −→ ẋi =
pi
mi
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The Hamiltonian is found by:

H =
∑
i

piẋi − L = T + V =
p21
2m

+
p22
2m

+
1

2
k(x21 + x22) +

1

2
k(x1 − x2)

2

Solving Hamilton’s equations gives the equations of motion:

∂H
∂pi

= ẋi −→ ẋi =
pi
mi

−∂H
∂xi

= ṗi −→ ṗ1 = −2kx1 + kx2, ṗ2 = kx1 − 2kx2

But ṗi = mẍi, so we get the same equations of motion as befroe:

mẍ1 = −2kx1 + kx2, mẍ2 = kx1 − 2kx2

Exercise 8. The Lagrangian is:

L =
1

2
(m1 +m2) |ṙCM|2 + 1

2

m1m2

m1 +m2
|ṙ|2 − V (r)

The generalised momenta are:

pCM =
∂L
∂ṙCM

= (m1 +m2)|ṙCM|, p =
∂L
∂ṙ

=

(
m1m2

m1 +m2

)
|ṙ|

Writing m1 +m2 =M and m1m2/M = µ, and finding the Hamiltonian:

H =
∑
i

piq̇i − L =
1

2
M
∣∣∣pCM

M

∣∣∣2 + 1

2
µ

∣∣∣∣ rµ
∣∣∣∣2 + V (r) =

|pCM|
2M

+
|p|2

2µ
+ V (r)

Exercise 9.

{ω, λ} =
∑
i

(
∂ω

∂qi

∂λ

∂pi
− ∂ω

∂pi

∂λ

∂qi

)

{λ, ω} =
∑
i

(
∂λ

∂qi

∂ω

∂pi
− ∂λ

∂pi

∂ω

∂qi

)
= −{ω, λ}

{ω, λ+ σ} =
∑
i

(
∂ω

∂qi

∂(λ+ σ)

∂pi
− ∂ω

∂pi

∂(λ+ σ)

∂qi

)
=

∑
i

(
∂ω

∂qi

∂λ

∂pi
− ∂ω

∂pi

∂λ

∂qi

)
+
∑
i

(
∂ω

∂qi

∂σ

∂pi
− ∂ω

∂pi

∂σ

∂qi

)
= {ω, λ}+ {ω, σ}

{ω, λσ} =
∑
i

(
∂ω

∂qi

∂λσ

∂pi
− ∂ω

∂pi

∂λσ

∂qi

)
=

∑
i

σ

(
∂ω

∂qi

∂λ

∂pi
− ∂ω

∂pi

∂λ

∂qi

)
+
∑
i

λ

(
∂ω

∂qi

∂σ

∂pi
− ∂ω

∂pi

∂σ

∂qi

)
= {ω, λ}σ + λ{ω, σ}
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Exercise 10. (i)

{qi, qj} =
∑
k

(
∂qi
∂qk

∂qj
∂pk

− ∂qi
∂pk

∂qj
∂qk

)
= 0, ∵ ∂qi

∂qk
= δik,

∂qj
∂qk

= δjk, ∀ i, j, k ∈ N

{pi, pj} =
∑
k

(
∂pi
∂qk

∂pj
∂pk

− ∂pi
∂pk

∂pj
∂qk

)
= 0, ∵ ∂pi

∂pk
= δik,

∂pj
∂pk

= δjk, ∀ i, j, k ∈ N

(ii) The Hamiltonian with a = b is:

H = p2x + p2y + a(x2 + y2)

The angular momentum about the z-axis lz = xpy − ypx is conserved because the potential V (x, y) is
expressible as V (x2+ y2) and the z-coordinate is not present in the Hamiltonian. Explicit computation yields:

{lz,H} =
∑
i

(
∂lz
∂qi

∂H
∂pi

− ∂lz
∂pi

∂H
∂qi

)
=

(
∂lz
∂x

∂H
∂px

− ∂lz
∂px

∂H
∂x

)
+

(
∂lz
∂y

∂H
∂py

− ∂lz
∂py

∂H
∂y

)
= (py · 2px − y · 2x) + (−px · 2py − (−px) · 2y) = 0

Exercise 11.

Exercise 12.

{x̄, ȳ} =
∑

k=x,y

(
∂x̄

∂qk

∂ȳ

∂pk
− ∂x̄

∂pk

∂ȳ

∂qk

)
= 0

{x̄, p̄y} =
∑

k=x,y

(
∂x̄

∂qk

∂p̄y
∂pk

− ∂x̄

∂pk

∂p̄y
∂qk

)
= 0

Exercise 13.

{ρ, pρ} =
∑

k=x,y

(
∂ρ

∂qk

∂pρ
∂pk

− ∂ρ

∂pk

∂pρ
∂qk

)
=

(
x√

x2 + y2

)2

+

(
y√

x2 + y2

)2

= 1

{ρ, pϕ,=}
∑

k=x,y

(
∂ρ

∂qk

∂pϕ
∂pk

− ∂ρ

∂pk

∂pϕ
∂qk

)
= −y

(
x√

x2 + y2

)
+ x

(
y√

x2 + y2

)
= 0

{ϕ, pρ} =
∑

k=x,y

(
∂ϕ

∂qk

∂pρ
∂pk

− ∂ϕ

∂pk

∂pρ
∂qk

)
=

(
−y

x2 + y2

)(
x√

x2 + y2

)

+

(
x

x2 + y2

)(
y√

x2 + y2

)
= 0

{ϕ, pϕ} =
∑

k=x,y

(
∂ϕ

∂qk

∂pϕ
∂pk

− ∂ϕ

∂pk

∂pϕ
∂qk

)
= −y

(
−y

x2 + y2

)
+ x

(
x

x2 + y2

)
= 1

{ρ, ϕ} =
∑

k=x,y

(
∂ρ

∂qk

∂ϕ

∂pk
− ∂ρ

∂pk

∂ϕ

∂qk

)
= 0

{pρ, pϕ} =
∑

k=x,y

(
∂pρ
∂qk

∂pϕ
∂pk

− ∂pρ
∂pk

∂pϕ
∂qk

)
= 0
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Exercise 14.

Exercise 15.

Exercise 16.

Exercise 17. All we have to do is check the infinitesimal changes for p = p1 + p2:

δx1 = ϵ
∂p

∂p1
= ϵ, δx2 = ϵ

∂p

∂p2
= ϵ

δp1 = −ϵ ∂p
∂x1

= 0, δp2 = −ϵ ∂p
∂x2

= 0

Therefore, the generator g(q, p) = p.

Exercise 18. The infinitesimal transformations are:

q̄i = qi + ϵ
∂g

∂pi
, p̄j = pj − ϵ

∂g

∂qj

Checking the Poisson brackets:

{q̄i, p̄j} =
∑
k

(
∂q̄i
∂qk

∂q̄j
∂pk

− ∂q̄i
∂pk

∂p̄j
∂qk

)
=

∑
k

[(
δik + ϵ

∂2g

∂pi∂qk

)(
δjk − ϵ

∂2g

∂qj∂pk

)
−
(
ϵ
∂2g

∂pi∂pk

)(
−ϵ ∂2g

∂qi∂qk

)]
=
∑
k

[
δikδjk + ϵδjk

∂2g

∂pi∂qk
− ϵδik

∂2g

∂qj∂pk
+ ϵ2

∂2g

∂pi∂pk

∂2g

∂qi∂qk

]
= δij + ϵ

(
∂2g

∂pi∂qj
− ∂2g

∂qj∂pi

)
+O

(
ϵ2
)
= δij , ∵ ∂2g

∂pi∂qj
=

∂2g

∂qj∂pi
, O

(
ϵ2
)
≈ 0

Exercise 19. The Hamiltonian under rotated coordinates is:

HR =
p2x + p2y
2m

+
1

2
mω2[(x cos θ − y sin θ)2 + (x sin θ + y cos θ)2] = H

For the transformation to be noncanonical, the Poisson bracket {x̄, p̄x} ̸= 1:

{x̄, p̄x} =
∑

k=x,y

(
∂x̄

∂qk

∂p̄x
∂pk

− ∂x̄

∂pk

∂p̄x
∂qk

)
= cos θ

To show that no conservation law follows:

q̄i = qi + ϵ
∂g

∂pi
= qi + δqi, p̄i = pi → δpi = 0

δH =
∑
i

∂H
∂qi

(
ϵ
∂g

∂pi

)
̸= ϵ{H, g}

Exercise 20. A rotation in phase space can be shown via the following diagram:
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x

p

x̄

p̄

The infinitesimal transformation is as follows:

x̄ = x cos ϵ− p sin ϵ ≈ x− ϵp

p̄ = x sin ϵ+ p cos ϵ ≈ ϵx+ p

We must verify if this transformation is canonical:

{x̄, p̄} =
∑

k=x,p

(
∂x̄

∂qk

∂p̄

∂pk
− ∂x̄

∂pk

∂p̄

∂qk

)
= 0

To find the generator, we must solve the following partial differential equations:

∂g

∂p
= −p −→ g = −p

2

2
+ f(x)

∂g

∂x
= −x −→ g = −x

2

2
+ h(p)

∴ g = −
(
p2

2
+
x2

2

)
= −H, so the generator is the negative of the Hamiltonian!

Exercise 21.



Chapter 3

The Postulates - A General Discussion

Exercise 1. (1) The possible values are the eigenvalues of Lz. Since Lz is already diagonal, its eigenvalues
are the diagonal elements 1, 0 and -1.

(2)

⟨Lx⟩ = ⟨1|Lx|1⟩ =
[
1 0 0

] 1√
2

0 1 0
1 0 1
0 1 0

10
0

 = 0

⟨
L2
x

⟩
= ⟨1|L2

x|1⟩ =
[
1 0 0

] 1
2

1 0 1
0 2 0
1 0 1

10
0

 =
1

2

∆Lx =

√
⟨L2

x⟩ − ⟨Lx⟩2 =
1√
2

(3) We must solve the eigenvalue problem for Lx:

1√
2

∣∣∣∣∣∣
−λ 1 0
1 −λ 1
0 1 −λ

∣∣∣∣∣∣ = 1√
2
[−λ(λ2 − 1)− (−λ)] = 0 −→ λ = 1, 0,−1

The eigenstates are found by substituting the eigenvalues and solving:

|Lx = 0⟩ = 1√
2

 1
0
−1

 , |Lx = 1⟩ = 1√
2

1/√2
1

1/
√
2

 , |Lx = −1⟩ = 1√
2

1/√2
−1

1/
√
2


(4) The eigenstate |ψ⟩ for the eigenvalue Lz = −1 is:

|ψ⟩ =

00
1



9



10

The probabilities are found by dotting the ket with the eigenbras corresponding to the eigenstates of Lz:

P (Lx = 0) = | ⟨Lx = 0|ψ⟩ |2 =

∣∣∣∣∣∣ 1√
2

[
1 0 −1

] 00
1

∣∣∣∣∣∣
2

=
1

2

P (Lx = 1) = | ⟨Lx = 1|ψ⟩ |2 =

∣∣∣∣∣∣ 1√
2

[
1√
2

1 1√
2

]00
1

∣∣∣∣∣∣
2

=
1

4

P (Lx = −1) = | ⟨Lx = −1|ψ⟩ |2 =

∣∣∣∣∣∣ 1√
2

[
1√
2

−1 1√
2

]00
1

∣∣∣∣∣∣
2

=
1

4

(5) L2
z is a degenerate matrix with eigenvalues 0, 1, 1, so when the state is measured to be L2

z = 1, the state
after the measurement is an eigenspace in V2. The linearly independent eigenkets describing this eigenspace
corresponding to the eigenvalue L2

z = 1 are:

|ω, 1⟩ =

10
0

 , |ω, 2⟩ =

00
1


Constructing the projection operator for these eigenkets to find the normalised state and its probability after
measurement:

Pω =
∑
i

|ω, i⟩⟨ω, i|

|ψ′⟩ = Pω |ψ⟩
|⟨Pωψ|Pωψ⟩|

=
2√
3

 1/2
0

1/
√
2


P
(
L2
z = 1

)
= ⟨ψ|Pω|ψ⟩ =

⟨[
1
2

1
2

1√
2

]∣∣∣∣∣∣
10
0

 [1 0 0
]
+

00
1

 [0 0 1
]∣∣∣∣∣∣
 1/2

1/2

1/
√
2

⟩

=
[
1
2

1
2

1√
2

]1 0 0
0 0 0
0 0 1

 1/2
1/2

1/
√
2

 =
3

4

The outcomes of measuring Lz are its eigenvalues, which are ω1 = 0, ω2 = 1, ω3 = −1. Their respective
probabilities are found by dotting the current state with their eigenvectors:

P (Lz = 0) = |⟨ω1|ψ′⟩|2 =

[0 1 0
] 2√

3

 1/2
0

1/
√
2

2

= 0

P (Lz = 1) = |⟨ω2|ψ′⟩|2 =

[1 0 0
] 2√

3

 1/2
0

1/
√
2

2

=
1

3

P (Lz = −1) = |⟨ω3|ψ′⟩|2 =

[0 0 1
] 2√

3

 1/2
0

1/
√
2

2

=
2

3
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(6) The probabilities for each of the eigenvalues of Lz is:

P (Lz = 0) = |⟨ω1|ψ⟩|2 =
1

2
= |α|2

P (Lz = 1) = |⟨ω2|ψ⟩|2 =
1

4
= |β|2

P (Lz = 1) = |⟨ω3|ψ⟩|2 =
1

4
= |γ|2

The normalised state is thus:

|ψ⟩ = α |Lz = 0⟩+ β |Lz = 1⟩+ γ |Lz = −1⟩√
|α|2 + |β|2 + |γ|2

= α |Lz = 0⟩+ β |Lz = 1⟩+ γ |Lz = −1⟩

However, the most general state is:

|ψ⟩ = eiδ1√
2
|Lz = 0⟩+ eiδ2

2
|Lz = 1⟩+ eiδ3

2
|Lz = −1⟩

This is because when performing measurements of other variables, interference terms come into play. For
example, if we measure Lx = 0 in the given state:

P (Lx = 0) = |⟨Lx = 0|ψ⟩|2 =

∣∣∣∣∣∣ 1√
2

[
1 0 −1

] 1
2

 eiδ1√
2eiδ2

eiδ3

∣∣∣∣∣∣
2

=
1

2
sin2

(
δ3 − δ1

2

)

Evidently the state will depend on the phase difference (δ3 − δ1). Clearly the exponential phase factors are
relevant in measuring probabilities.

Exercise 2. The expectation value is given by:

⟨P ⟩ = ⟨ψ|P |ψ⟩ =
∫ ∞

−∞
⟨ψ|k⟩ ⟨k|P |ψ⟩ dk =

∫ ∞

−∞
pψ∗(k)ψ(k) dk

ψ(k) = ⟨k|ψ⟩ =
∫ ∞

−∞
⟨k|x⟩ ⟨x|ψ⟩dx =

1√
2π

∫ ∞

−∞
e−ikxψ(x) dx

ψ∗(k) =
1√
2π

∫ ∞

−∞
eikxψ∗(x) dx = ψ(−k), ∵ ψ∗(x) = ψ(x)

⟨P ⟩ =
∫ ∞

−∞
ℏk ψ(−k)ψ(k) dk = 0, ∵ the integral is odd

Exercise 3.

Exercise 4.



Chapter 4

Simple Problems in One Dimension

Exercise 1. This can be solved by substitution:

p = ±
√
2mE −→ dp = ± m√

2mE
dE

Since there are two values that p can take, we must expand the integral to include the values with respect to
E:

U(t) =

∫ 0

−∞
− m√

2mE
|E,−⟩⟨E,−| e−iEt/ℏ dE +

∫ ∞

0

m√
2mE

|E,+⟩⟨E,+| e−iEt/ℏ dE

U(t) =
∑
α=±

∫ ∞

0

m√
2mE

|E,α⟩⟨E,α| e−iEt/ℏ dE

Exercise 2. Using |x⟩ as a trial solution:

P 2

2m
|x⟩ = E |x⟩

− ℏ2

2m

∂2

∂x2
|x⟩ = E |x⟩(

ℏ2

2m

d2

dx2
+ E

)
|x⟩ = 0

The solution to this differential equation is readily found by substituting D = d
dx and solving the algebraic

equation, giving:

D = ± ip
ℏ

−→ ψE(x) =
β√
2πℏ

exp

(
ip

ℏ
x

)
+

γ√
2πℏ

exp

(
− ip

ℏ
x

)
, p =

√
2mE

If E ≤ 0, then the function consists of real exponentials that blow up at large values of x, and are thus not
in the Hilbert space.
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Exercise 3. We have the propagator and initial state:

U(t) = exp

[
i

ℏ

(
ℏ2t
2m

d2

dx2

)]
=

∞∑
n=0

1

n!

(
iℏt
2m

)n
d2n

dx2n
, ψ(x, 0) =

e−x2/2

4
√
π

Expanding the initial state as a power series: ψ(x, 0) =
1
4
√
π

∞∑
n=0

(−1)nx2n

n!(2)n

ψ(x, t) =

( ∞∑
k=0

1

k!

(
iℏt
2m

)k
d2k

dx2k

)( ∞∑
n=0

1
4
√
π

(−1)nx2n

n!(2)n

)

ψ(x, t) =
1
4
√
π

[ ∞∑
n=0

n∑
k=0

(
iℏt
m

)k
(−1)

n

n!k!(2)n+k

(2n)!

(2n− 2k)!
x2(n−k)

]

The coefficients of the x2n terms are:

x0 :
(−1)0

0!

[
1− 1

2

iℏt
m

+
3

8

(
iℏt
m

)2

− 5

16

(
iℏt
m

)3

+
35

128

(
iℏt
m

)4

− ...

]
x2×0

20

x2 :
(−1)1

1!

[
1− 3

2

(
iℏt
m

)
+

15

8

(
iℏt
m

)2

− 35

16

(
iℏt
m

)3

+ ...

]
x2×1

21

x4 :
(−1)2

2!

[
1− 5

2

(
iℏt
m

)
+

35

8

(
iℏt
m

)2

− ...

]
x2×2

22

ψ(x, t) =
1
4
√
π

[ ∞∑
n=0

(−1)n

n!

{
1−

(
n+

1

2

)(
iℏt
m

)
+

1

2!

(
n+

1

2

)(
n+

3

2

)(
iℏt
m

)2

− ...

}
x2n

2n

]

ψ(x, t) =
1
4
√
π

[ ∞∑
n=0

(−1)n

n!

(
1 +

iℏt
m

)−n− 1
2 x2n

2n

]

=
1√√

π
(
1 + iℏt

m

) exp
[
− x2

2
(
1 + iℏt

m

)]

Exercise 4.
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